\documentclass{article}
\usepackage{amsmath}
\usepackage{amssymb}
\usepackage{amsthm}
\usepackage{geometry}
\geometry{margin=1in}

\title{Solving $f' = f$ Using Completely Rigorous Methods}
\author{}
\date{}

\begin{document}
\maketitle

We want to solve the differential equation:
\[ f' = f \]

First, rewrite this in terms of the integration operator:
\[ f = \int f \]

Subtract $\int f$ from both sides and factor out $f$:
\[ f - \int f = 0 \quad\Longrightarrow\quad \left(1 - \int\right) f = 0 \]

I'm not allowed to do this, but I'm going to do it anyway.
\[ f = (1 - \int)^{-1} 0 \]

Using the geometric series formula:
\[ (1-x)^{-1} = 1 + x + x^2 + x^3 + \cdots \]

We apply this to our integration operator:
\[ f = \left(1 + \int + \int\int + \int\int\int + \cdots\right) 0 \]

Evaluating term by term:
\begin{align*}
1 \cdot 0 &= 0 \\
\int 0 &= C \\
\int\int 0 &= Cx \\
\int\int\int 0 &= C\frac{x^2}{2!} \\
\int\int\int\int 0 &= C\frac{x^3}{3!} \\
&\vdots
\end{align*}

Adding these up gives us:
\[ f = 0 + C + Cx + C\frac{x^2}{2!} + C\frac{x^3}{3!} + \cdots \]

This is exactly the Taylor series for $Ce^x$! Therefore:
\[ f(x) = Ce^x \]

No, this is not a rigorous proof. It is a fake proof that leads to the correct answer.

\end{document}